Refactor Logic

Logic/Propositional/Linear/Intuitionistic.lean
@@ -24,78 +24,14 @@ theorem Ctx.nil_append : ∀ {Γ}, nil.append Γ = Γ
   | nil => rfl
   | cons .. => congrArg (cons · _) nil_append
 
-theorem Ctx.append_append : ∀ {Γ''}, append Γ (append Γ' Γ'') = append (append Γ Γ') Γ''
+theorem Ctx.append_append : ∀ {Γ''}, append Γ (Γ'.append Γ'') = (Γ.append Γ').append Γ''
   | nil => rfl
   | cons .. => congrArg (cons · _) append_append
 
-inductive Mem (A : Propn) : (Γ : Ctx) → Type
-  | here : Mem A (.cons Γ A)
-  | there (u : Mem A Γ) : Mem A (Γ.cons B)
-
-def Ctx.del : ∀ {Γ}, (u : Mem A Γ) → Ctx
-  | cons Γ _, .here => Γ
-  | cons Γ A, .there u => (Γ.del u).cons A
-
-def Mem.ofMemDel : {u : Mem B Γ} → (v : Mem A (Γ.del u)) → Mem A Γ
-  | here, v => there v
-  | there (B := .(A)) (Γ := Γ) u, here => here
-  | there (B := C) (Γ := Γ) u, there v => (ofMemDel v).there
-
-def Mem.del : (u : Mem A Γ) → (v : Mem B (Γ.del u)) → Mem A (Γ.del (ofMemDel v))
-  | here, _ => here
-  | there (B := .(B)) (Γ := Γ) u, here => u
-  | there (B := C) (Γ := Γ) u, there v => (u.del v).there
-
-theorem Ctx.del_del : {u : Mem A Γ} → (v : Mem B (Γ.del u)) → (Γ.del u).del v = (Γ.del (.ofMemDel v)).del (u.del v)
-  | .here, _ => rfl
-  | .there (B := .(B)) (Γ := Γ) u, .here => rfl
-  | .there (B := C) (Γ := Γ) u, .there v => congrArg (cons · C) (del_del v)
-
-inductive Rename : (Γ Γ' : Ctx) → Type
-  | nil : Rename .nil .nil
-  | cons (u : Mem A Γ') (γ : Rename Γ (Γ'.del u)) : Rename (Γ.cons A) Γ'
-
-def Rename.cons' (γ : Rename Γ Γ') {A} : Rename (Γ.cons A) (Γ'.cons A) :=
-  cons .here γ
-
-def Rename.consAppend : ∀ {Γ₂}, (γ : Rename (.append Γ₁ Γ₂) Γ') → Rename ((Γ₁.cons A).append Γ₂) (Γ'.cons A)
-  | .nil, γ => γ.cons'
-  | .cons .., cons u γ => cons u.there γ.consAppend
-
-def Rename.append (γ : Rename (.append Γ₁ Γ₂) Γ') : ∀ {Γ}, Rename ((Γ₁.append Γ).append Γ₂) (Γ'.append Γ)
-  | .nil => γ
-  | .cons .. => γ.append.consAppend
-
-def Rename.id : ∀ {Γ}, Rename Γ Γ
-  | .nil => nil
-  | .cons .. => id.cons'
-
-def Rename.exchange : Rename (Ctx.cons Γ A |>.cons B) (Γ.cons B |>.cons A) :=
-  cons (.there .here) id
-
-def Rename.exchange₂ : Rename (Ctx.cons Γ A |>.cons B |>.cons C) (Γ.cons B |>.cons C |>.cons A) :=
-  cons (.there .here) (cons (.there .here) id)
-
-def Rename.appendSwap : ∀ {Γ₁}, Rename (.append Γ₁ Γ₂) (Γ₂.append Γ₁)
-  | .nil => Ctx.nil_append ▸ .id
-  | .cons .. => consAppend appendSwap
-
-def Mem.rename : (γ : Rename Γ Γ') → ∀ {A}, (u : Mem A Γ) → Mem A Γ'
-  | .cons u _, _, here => u
-  | .cons _ γ, _, there u => ofMemDel (u.rename γ)
-
-def Rename.del : (γ : Rename Γ Γ') → ∀ {A}, (u : Mem A Γ) → Rename (Γ.del u) (Γ'.del (u.rename γ))
-  | cons _ γ, _, .here => γ
-  | cons u' γ, _, .there u => cons (u'.del (u.rename γ)) (Ctx.del_del (u.rename γ) ▸ γ.del u)
-
-def Rename.comp : (γ : Rename Γ Γ') → (γ' : Rename Γ' Γ'') → Rename Γ Γ''
-  | nil, γ' => γ'
-  | cons u γ, γ' => cons (u.rename γ') (γ.comp (γ'.del u))
-
 inductive Split : (Γ Γ₁ Γ₂ : Ctx) → Type
   | nil : Split .nil .nil .nil
-  | cons₁ (h : Split Γ Γ₁ Γ₂) : Split (Γ.cons A) (Γ₁.cons A) Γ₂
-  | cons₂ (h : Split Γ Γ₁ Γ₂) : Split (Γ.cons A) Γ₁ (Γ₂.cons A)
+  | cons₁ (s : Split Γ Γ₁ Γ₂) : Split (Γ.cons A) (Γ₁.cons A) Γ₂
+  | cons₂ (s : Split Γ Γ₁ Γ₂) : Split (Γ.cons A) Γ₁ (Γ₂.cons A)
 
 def Split.triv₁ : ∀ {Γ}, Split Γ Γ .nil
   | .nil => nil
@@ -105,89 +41,105 @@ def Split.triv₂ : ∀ {Γ}, Split Γ .nil Γ
   | .nil => nil
   | .cons .. => triv₂.cons₂
 
-theorem Split.eq_triv₁ : ∀ h, (⟨Γ₁, h⟩ : Σ Γ₁, Split Γ Γ₁ _) = ⟨Γ, .triv₁⟩
+theorem Split.eq_triv₁ : ∀ s, (⟨Γ₁, s⟩ : Σ Γ₁, Split Γ Γ₁ .nil) = ⟨Γ, triv₁⟩
   | nil => rfl
-  | cons₁ h => match h.eq_triv₁ with | rfl => rfl
+  | cons₁ s => let .refl _ := s.eq_triv₁; rfl
 
-theorem Split.eq_triv₂ : ∀ h, (⟨Γ₂, h⟩ : Σ Γ₂, Split Γ _ Γ₂) = ⟨Γ, .triv₂⟩
+theorem Split.eq_triv₂ : ∀ s, (⟨Γ₂, s⟩ : Σ Γ₂, Split Γ .nil Γ₂) = ⟨Γ, triv₂⟩
   | nil => rfl
-  | cons₂ h => match h.eq_triv₂ with | rfl => rfl
+  | cons₂ s => let .refl _ := s.eq_triv₂; rfl
 
-def Split.flip : (h : Split Γ Γ₁ Γ₂) → Split Γ Γ₂ Γ₁
+def Split.flip : (s : Split Γ Γ₁ Γ₂) → Split Γ Γ₂ Γ₁
   | nil => nil
-  | cons₁ h => h.flip.cons₂
-  | cons₂ h => h.flip.cons₁
+  | cons₁ s => s.flip.cons₂
+  | cons₂ s => s.flip.cons₁
 
-def Split.shift₁ : (h : Split Γ Γ₁ Γ₂) → (h₁ : Split Γ₁ Γ₁₁ Γ₁₂) → Σ Γ', Split Γ Γ₁₁ Γ' × Split Γ' Γ₁₂ Γ₂
-  | h, nil => ⟨Γ, triv₂, h⟩
-  | cons₁ h, cons₁ h₁ => let ⟨Γ', h', h''⟩ := h.shift₁ h₁; ⟨Γ', h'.cons₁, h''⟩
-  | cons₁ h, cons₂ h₁ => let ⟨Γ', h', h''⟩ := h.shift₁ h₁; ⟨Γ'.cons _, h'.cons₂, h''.cons₁⟩
-  | cons₂ h, h₁ => let ⟨Γ', h', h''⟩ := h.shift₁ h₁; ⟨Γ'.cons _, h'.cons₂, h''.cons₂⟩
+def Split.shift₁ : (s : Split Γ Γ₁ Γ₂) → (s₁ : Split Γ₁ Γ₁₁ Γ₁₂) → Σ Γ', Split Γ Γ₁₁ Γ' × Split Γ' Γ₁₂ Γ₂
+  | s, nil => ⟨_, triv₂, s⟩
+  | cons₁ s, cons₁ s₁ => let ⟨_, s, s'⟩ := s.shift₁ s₁; ⟨_, s.cons₁, s'⟩
+  | cons₁ s, cons₂ s₁ => let ⟨_, s, s'⟩ := s.shift₁ s₁; ⟨_, s.cons₂, s'.cons₁⟩
+  | cons₂ s, s₁ => let ⟨_, s, s'⟩ := s.shift₁ s₁; ⟨_, s.cons₂, s'.cons₂⟩
 
-def Split.shift₂ : (h : Split Γ Γ₁ Γ₂) → (h₂ : Split Γ₂ Γ₂₁ Γ₂₂) → Σ Γ', Split Γ Γ' Γ₂₂ × Split Γ' Γ₁ Γ₂₁
-  | h, nil => ⟨Γ, triv₁, h⟩
-  | cons₂ h, cons₁ h₂ => let ⟨Γ', h', h''⟩ := h.shift₂ h₂; ⟨Γ'.cons _, h'.cons₁, h''.cons₂⟩
-  | cons₂ h, cons₂ h₂ => let ⟨Γ', h', h''⟩ := h.shift₂ h₂; ⟨Γ', h'.cons₂, h''⟩
-  | cons₁ h, h₂ => let ⟨Γ', h', h''⟩ := h.shift₂ h₂; ⟨Γ'.cons _, h'.cons₁, h''.cons₁⟩
-
-def Split.ofMem : (u : Mem A Γ) → Split Γ (.cons .nil A) (Γ.del u)
-  | .here => triv₂.cons₁
-  | .there u => (ofMem u).cons₂
-
-def Split.rename : (h : Split Γ Γ₁ Γ₂) → Rename (Γ₁.append Γ₂) Γ
-  | nil => .nil
-  | cons₁ h => h.rename.consAppend
-  | cons₂ h => .cons .here h.rename
-
-def Rename.split : (γ : Rename Γ Γ') → ∀ {Γ₁ Γ₂}, (h : Split Γ Γ₁ Γ₂) → Σ Γ₁' Γ₂', Rename Γ₁ Γ₁' × Rename Γ₂ Γ₂' × Split Γ' Γ₁' Γ₂'
-  | nil, _, _, .nil => ⟨.nil, .nil, nil, nil, .nil⟩
-  | cons u γ, _, _, .cons₁ h => let ⟨_, Γ₂', γ₁, γ₂, h⟩ := γ.split h; let ⟨Γ₁', h, h'⟩ := (Split.ofMem u).shift₂ h; ⟨Γ₁', Γ₂', γ₁.cons'.comp h'.flip.rename, γ₂, h⟩
-  | cons u γ, _, _, .cons₂ h => let ⟨Γ₁', _, γ₁, γ₂, h⟩ := γ.split h; let ⟨Γ₂', h, h'⟩ := (Split.ofMem u).flip.shift₁ h; ⟨Γ₁', Γ₂', γ₁, γ₂.cons'.comp h'.rename, h⟩
-
-def Mem.ofSplit₁ : (u : Mem A Γ₁) → (h : Split Γ Γ₁ Γ₂) → Mem A Γ
-  | here, .cons₁ _ => here
-  | there u, .cons₁ h | u, .cons₂ h => (u.ofSplit₁ h).there
-
-def Mem.ofSplit₂ : (u : Mem A Γ₂) → (h : Split Γ Γ₁ Γ₂) → Mem A Γ
-  | here, .cons₂ h => here
-  | there u, .cons₂ h | u, .cons₁ h => (u.ofSplit₂ h).there
-
-def Split.del₁ : (u : Mem A Γ₁) → (h : Split Γ Γ₁ Γ₂) → Split (Γ.del (u.ofSplit₁ h)) (Γ₁.del u) Γ₂
-  | .here, cons₁ h => h
-  | .there u, cons₁ h => (h.del₁ u).cons₁
-  | .here, cons₂ h | .there _, cons₂ h => (h.del₁ _).cons₂
-
-def Split.del₂ : (u : Mem A Γ₂) → (h : Split Γ Γ₁ Γ₂) → Split (Γ.del (u.ofSplit₂ h)) Γ₁ (Γ₂.del u)
-  | .here, cons₂ h => h
-  | .there u, cons₂ h => (h.del₂ u).cons₂
-  | .here, cons₁ h | .there _, cons₁ h => (h.del₂ _).cons₁
-
-def Split.append : ∀ {Γ₂}, Split (Γ₁.append Γ₂) Γ₁ Γ₂
+def Split.mkAppend : ∀ {Γ₂}, Split (Γ₁.append Γ₂) Γ₁ Γ₂
   | .nil => triv₁
-  | .cons .. => append.cons₂
+  | .cons .. => mkAppend.cons₂
 
-class Judge (J : (Γ : Ctx) → (A : Propn) → Type) where
-  hyp : J (.cons .nil A) A
+def Split.append₂ (s : Split Γ Γ₁ Γ₂) : ∀ {Γ'}, Split (Γ.append Γ') Γ₁ (Γ₂.append Γ')
+  | .nil => s
+  | .cons .. => s.append₂.cons₂
+
+def Split.append₂' : (s : Split Γ Γ₁ Γ₂) → ∀ {Γ'}, Split (.append Γ' Γ) Γ₁ (Γ'.append Γ₂)
+  | nil => triv₂
+  | cons₁ s => s.append₂'.cons₁
+  | cons₂ s => s.append₂'.cons₂
 
 inductive Subst (J : (Γ : Ctx) → (A : Propn) → Type) : (Γ Γ' : Ctx) → Type
   | nil : Subst J .nil .nil
-  | cons (h : Split Γ' Γ₁ Γ₂) (D : J Γ₁ A) (γ : Subst J Γ Γ₂) : Subst J (Γ.cons A) Γ'
+  | cons (s : Split Γ' Γ₁ Γ₂) (D : J Γ₁ A) (γ : Subst J Γ Γ₂) : Subst J (Γ.cons A) Γ'
 
-def Subst.cons' [Judge J] : (γ : Subst J Γ Γ') → Subst J (Γ.cons A) (Γ'.cons A) :=
-  cons (.cons₁ .triv₂) Judge.hyp
+def Subst.split : (γ : Subst J Γ Γ') → ∀ {Γ₁ Γ₂}, (s : Split Γ Γ₁ Γ₂) → Σ Γ₁' Γ₂', Split Γ' Γ₁' Γ₂' × Subst J Γ₁ Γ₁' × Subst J Γ₂ Γ₂'
+  | nil, _, _, .nil => ⟨_, _, .nil, nil, nil⟩
+  | cons s' D γ, _, _, .cons₁ s => let ⟨_, _, s, γ₁, γ₂⟩ := γ.split s; let ⟨_, s, s'⟩ := s'.flip.shift₁ s.flip; ⟨_, _, s.flip, cons s'.flip D γ₁, γ₂⟩
+  | cons s' D γ, _, _, .cons₂ s => let ⟨_, _, s, γ₁, γ₂⟩ := γ.split s; let ⟨_, s, s'⟩ := s'.flip.shift₁ s; ⟨_, _, s, γ₁, cons s'.flip D γ₂⟩
 
-def Subst.id [Judge J] : ∀ {Γ}, Subst J Γ Γ
+def Subst.append (γ₁ : Subst J Γ₁ Γ₁') : (γ₂ : Subst J Γ₂ Γ₂') → Subst J (Γ₁.append Γ₂) (Γ₁'.append Γ₂')
+  | nil => γ₁
+  | cons s D γ₂ => cons s.append₂' D (γ₁.append γ₂)
+
+def Subst.consAppend (D : J (.cons .nil A) A) : ∀ {Γ₂}, (γ : Subst J (.append Γ₁ Γ₂) Γ') → Subst J ((Γ₁.cons A).append Γ₂) (Γ'.cons A)
+  | .nil, γ => cons (.cons₁ .triv₂) D γ
+  | .cons .., cons s D' γ => cons s.cons₂ D' (γ.consAppend D)
+
+inductive Hyp : (Γ : Ctx) → (A : Propn) → Type
+  | mk : Hyp (.cons .nil A) A
+
+def Split.toSubst : (s : Split Γ Γ₁ Γ₂) → Subst Hyp (Γ₁.append Γ₂) Γ
+  | nil => .nil
+  | cons₁ s => .consAppend .mk s.toSubst
+  | cons₂ s => .cons triv₂.cons₁ .mk s.toSubst
+
+class JudgeTrans (J J' : (Γ : Ctx) → (A : Propn) → Type) where
+  transform (D : J Γ A) : J' Γ A
+
+instance JudgeTrans.id : JudgeTrans J J where
+  transform D := D
+
+abbrev Judge : (J : (Γ : Ctx) → (A : Propn) → Type) → Type :=
+  JudgeTrans Hyp
+
+def Subst.id [j : Judge J] : ∀ {Γ}, Subst J Γ Γ
   | .nil => nil
-  | .cons .. => id.cons'
+  | .cons .. => cons (.cons₁ .triv₂) (j.transform .mk) id
 
-def Subst.split : (γ : Subst J Γ Γ') → ∀ {Γ₁ Γ₂}, (h : Split Γ Γ₁ Γ₂) → Σ Γ₁' Γ₂', Subst J Γ₁ Γ₁' × Subst J Γ₂ Γ₂' × Split Γ' Γ₁' Γ₂'
-  | nil, _, _, .nil => ⟨.nil, .nil, nil, nil, .nil⟩
-  | cons h' D γ, _, _, .cons₁ h => let ⟨_, Γ₂', γ₁, γ₂, h⟩ := γ.split h; let ⟨Γ₁', h, h'⟩ := h'.shift₂ h; ⟨Γ₁', Γ₂', cons h' D γ₁, γ₂, h⟩
-  | cons h' D γ, _, _, .cons₂ h => let ⟨Γ₁', _, γ₁, γ₂, h⟩ := γ.split h; let ⟨Γ₂', h, h'⟩ := h'.flip.shift₁ h; ⟨Γ₁', Γ₂', γ₁, cons h'.flip D γ₂, h⟩
+def Subst.lift [j : Judge J] {Γ Γ' A} : (γ : Subst J Γ Γ') → Subst J (Γ.cons A) (Γ'.cons A) :=
+  cons (.cons₁ .triv₂) (j.transform .mk)
 
-def Subst.map (f : ∀ {Γ A}, J Γ A → J' Γ A) {Γ Γ'} : (γ : Subst J Γ Γ') → Subst J' Γ Γ'
+def Subst.map (jt : JudgeTrans J J') {Γ Γ'} : (γ : Subst J Γ Γ') → Subst J' Γ Γ'
   | nil => nil
-  | cons h D γ => cons h (f D) (γ.map f)
+  | cons s D γ => cons s (jt.transform D) (γ.map jt)
+
+def Subst.exchange : Subst Hyp (Ctx.cons Γ A |>.cons B) (Γ.cons B |>.cons A) :=
+  cons (.cons₂ (.cons₁ .triv₂)) .mk id
+
+def Subst.exchange₂ : Subst Hyp (Ctx.cons Γ A |>.cons B |>.cons C) (Γ.cons B |>.cons C |>.cons A) :=
+  cons (.cons₂ (.cons₁ .triv₂)) .mk exchange
+
+inductive Split₁ : (Γ : Ctx) → (A : Propn) → (Γ' : Ctx) → Type
+  | here : Split₁ (Γ.cons A) A Γ
+  | there (s : Split₁ Γ A Γ') : Split₁ (Γ.cons B) A (Γ'.cons B)
+
+def Split₁.toSplit : (s : Split₁ Γ A Γ') → Split Γ (.cons .nil A) Γ'
+  | here => .cons₁ .triv₂
+  | there s => s.toSplit.cons₂
+
+def Split₁.ofSplit : (s : Split Γ (.cons .nil A) Γ') → Split₁ Γ A Γ'
+  | .cons₁ s => let .refl _ := s.eq_triv₂; here
+  | .cons₂ s => (ofSplit s).there
+
+def Subst.split₁ (γ : Subst Hyp Γ Γ') {A Γ₂} (s : Split₁ Γ A Γ₂) : Σ Γ₂', Split₁ Γ' A Γ₂' × Subst Hyp Γ₂ Γ₂' :=
+  let ⟨_, _, s, cons s' .mk nil, γ⟩ := γ.split s.toSplit
+  let .cons₁ .nil := s'
+  ⟨_, .ofSplit s, γ⟩
 
 -- Natural Deduction
 namespace ND
@@ -195,56 +147,39 @@ namespace ND
 inductive True : (Γ : Ctx) → (A : Propn) → Type
   | hyp : True (.cons .nil A) A
   | oneI : True .nil .one
-  | oneE (h : Split Γ Γ₁ Γ₂) (D : True Γ₁ .one) (D₁ : True Γ₂ C) : True Γ C
-  | zeroE (h : Split Γ Γ₁ Γ₂) (D : True Γ₁ .zero) : True Γ C
+  | oneE (s : Split Γ Γ₁ Γ₂) (D : True Γ₁ .one) (D₁ : True Γ₂ C) : True Γ C
+  | zeroE (s : Split Γ Γ₁ Γ₂) (D : True Γ₁ .zero) : True Γ C
   | topI : True Γ .top
-  | tensorI (h : Split Γ Γ₁ Γ₂) (D₁ : True Γ₁ A) (D₂ : True Γ₂ B) : True Γ (A.tensor B)
-  | tensorE (h : Split Γ Γ₁ Γ₂) (D : True Γ₁ (A.tensor B)) (D₁ : True (Γ₂.cons A |>.cons B) C) : True Γ C
+  | tensorI (s : Split Γ Γ₁ Γ₂) (D₁ : True Γ₁ A) (D₂ : True Γ₂ B) : True Γ (A.tensor B)
+  | tensorE (s : Split Γ Γ₁ Γ₂) (D : True Γ₁ (A.tensor B)) (D₁ : True (Γ₂.cons A |>.cons B) C) : True Γ C
   | plusI₁ (D : True Γ A) : True Γ (A.plus B)
   | plusI₂ (D : True Γ B) : True Γ (.plus A B)
-  | plusE (h : Split Γ Γ₁ Γ₂) (D : True Γ₁ (A.plus B)) (D₁ : True (Γ₂.cons A) C) (D₂ : True (Γ₂.cons B) C) : True Γ C
+  | plusE (s : Split Γ Γ₁ Γ₂) (D : True Γ₁ (A.plus B)) (D₁ : True (Γ₂.cons A) C) (D₂ : True (Γ₂.cons B) C) : True Γ C
   | withI (D₁ : True Γ A) (D₂ : True Γ B) : True Γ (A.with B)
   | withE₁ (D : True Γ (A.with B)) : True Γ A
   | withE₂ (D : True Γ (.with A B)) : True Γ B
   | lolliI (D : True (Γ.cons A) B) : True Γ (A.lolli B)
-  | lolliE (h : Split Γ Γ₁ Γ₂) (D : True Γ₁ (A.lolli B)) (D₁ : True Γ₂ A) : True Γ B
+  | lolliE (s : Split Γ Γ₁ Γ₂) (D : True Γ₁ (A.lolli B)) (D₁ : True Γ₂ A) : True Γ B
 
-def True.rename (γ : Rename Γ Γ') {A} : (D : True Γ A) → True Γ' A
-  | hyp => let .cons u γ := γ; match u, γ with | .here (Γ := .nil), .nil => hyp
+instance True.judge : Judge True where
+  transform | .mk => hyp
+
+def True.subst [j : Judge J] [jt : JudgeTrans J True] {Γ Γ'} (γ : Subst J Γ Γ') {A} : (D : True Γ A) → True Γ' A
+  | hyp => let .cons s D .nil := γ; let .refl _ := s.eq_triv₁; jt.transform D
   | oneI => let .nil := γ; oneI
-  | oneE h D D₁ => let ⟨_, _, γ₁, γ₂, h⟩ := γ.split h; oneE h (D.rename γ₁) (D₁.rename γ₂)
-  | zeroE h D => let ⟨_, _, γ₁, _, h⟩ := γ.split h; zeroE h (D.rename γ₁)
+  | oneE s D D₁ => let ⟨_, _, s, γ₁, γ₂⟩ := γ.split s; oneE s (D.subst γ₁) (D₁.subst γ₂)
+  | zeroE s D => let ⟨_, _, s, γ₁, _⟩ := γ.split s; zeroE s (D.subst γ₁)
   | topI => topI
-  | tensorI h D₁ D₂ => let ⟨_, _, γ₁, γ₂, h⟩ := γ.split h; tensorI h (D₁.rename γ₁) (D₂.rename γ₂)
-  | tensorE h D D₁ => let ⟨_, _, γ₁, γ₂, h⟩ := γ.split h; tensorE h (D.rename γ₁) (D₁.rename γ₂.cons'.cons')
-  | plusI₁ D => plusI₁ (D.rename γ)
-  | plusI₂ D => plusI₂ (D.rename γ)
-  | plusE h D D₁ D₂ => let ⟨_, _, γ₁, γ₂, h⟩ := γ.split h; plusE h (D.rename γ₁) (D₁.rename γ₂.cons') (D₂.rename γ₂.cons')
-  | withI D₁ D₂ => withI (D₁.rename γ) (D₂.rename γ)
-  | withE₁ D => withE₁ (D.rename γ)
-  | withE₂ D => withE₂ (D.rename γ)
-  | lolliI D => lolliI (D.rename γ.cons')
-  | lolliE h D D₁ => let ⟨_, _, γ₁, γ₂, h⟩ := γ.split h; lolliE h (D.rename γ₁) (D₁.rename γ₂)
-
-instance True.instJudge : Judge True where
-  hyp := hyp
-
-def True.subst (γ : Subst True Γ Γ') {A} : (D : True Γ A) → True Γ' A
-  | hyp => let .cons h D .nil := γ; match h.eq_triv₁ with | rfl => D
-  | oneI => let .nil := γ; oneI
-  | oneE h D D₁ => let ⟨_, _, γ₁, γ₂, h⟩ := γ.split h; oneE h (D.subst γ₁) (D₁.subst γ₂)
-  | zeroE h D => let ⟨_, _, γ₁, _, h⟩ := γ.split h; zeroE h (D.subst γ₁)
-  | topI => topI
-  | tensorI h D₁ D₂ => let ⟨_, _, γ₁, γ₂, h⟩ := γ.split h; tensorI h (D₁.subst γ₁) (D₂.subst γ₂)
-  | tensorE h D D₁ => let ⟨_, _, γ₁, γ₂, h⟩ := γ.split h; tensorE h (D.subst γ₁) (D₁.subst γ₂.cons'.cons')
+  | tensorI s D₁ D₂ => let ⟨_, _, s, γ₁, γ₂⟩ := γ.split s; tensorI s (D₁.subst γ₁) (D₂.subst γ₂)
+  | tensorE s D D₁ => let ⟨_, _, s, γ₁, γ₂⟩ := γ.split s; tensorE s (D.subst γ₁) (D₁.subst γ₂.lift.lift)
   | plusI₁ D => plusI₁ (D.subst γ)
   | plusI₂ D => plusI₂ (D.subst γ)
-  | plusE h D D₁ D₂ => let ⟨_, _, γ₁, γ₂, h⟩ := γ.split h; plusE h (D.subst γ₁) (D₁.subst γ₂.cons') (D₂.subst γ₂.cons')
+  | plusE s D D₁ D₂ => let ⟨_, _, s, γ₁, γ₂⟩ := γ.split s; plusE s (D.subst γ₁) (D₁.subst γ₂.lift) (D₂.subst γ₂.lift)
   | withI D₁ D₂ => withI (D₁.subst γ) (D₂.subst γ)
   | withE₁ D => withE₁ (D.subst γ)
   | withE₂ D => withE₂ (D.subst γ)
-  | lolliI D => lolliI (D.subst γ.cons')
-  | lolliE h D D₁ => let ⟨_, _, γ₁, γ₂, h⟩ := γ.split h; lolliE h (D.subst γ₁) (D₁.subst γ₂)
+  | lolliI D => lolliI (D.subst γ.lift)
+  | lolliE s D D₁ => let ⟨_, _, s, γ₁, γ₂⟩ := γ.split s; lolliE s (D.subst γ₁) (D₁.subst γ₂)
 
 end ND
 
@@ -256,14 +191,14 @@ mutual
 inductive Verif : (Γ : Ctx) → (A : Propn) → Type
   | uv (D : Use Γ (.base P)) : Verif Γ (.base P)
   | oneI : Verif .nil .one
-  | oneE (h : Split Γ Γ₁ Γ₂) (D : Use Γ₁ .one) (D₁ : Verif Γ₂ C) : Verif Γ C
-  | zeroE (h : Split Γ Γ₁ Γ₂) (D : Use Γ₁ .zero) : Verif Γ C
+  | oneE (s : Split Γ Γ₁ Γ₂) (D : Use Γ₁ .one) (D₁ : Verif Γ₂ C) : Verif Γ C
+  | zeroE (s : Split Γ Γ₁ Γ₂) (D : Use Γ₁ .zero) : Verif Γ C
   | topI : Verif Γ .top
-  | tensorI (h : Split Γ Γ₁ Γ₂) (D₁ : Verif Γ₁ A) (D₂ : Verif Γ₂ B) : Verif Γ (A.tensor B)
-  | tensorE (h : Split Γ Γ₁ Γ₂) (D : Use Γ₁ (A.tensor B)) (D₁ : Verif (Γ₂.cons A |>.cons B) C) : Verif Γ C
+  | tensorI (s : Split Γ Γ₁ Γ₂) (D₁ : Verif Γ₁ A) (D₂ : Verif Γ₂ B) : Verif Γ (A.tensor B)
+  | tensorE (s : Split Γ Γ₁ Γ₂) (D : Use Γ₁ (A.tensor B)) (D₁ : Verif (Γ₂.cons A |>.cons B) C) : Verif Γ C
   | plusI₁ (D : Verif Γ A) : Verif Γ (A.plus B)
   | plusI₂ (D : Verif Γ B) : Verif Γ (.plus A B)
-  | plusE (h : Split Γ Γ₁ Γ₂) (D : Use Γ₁ (A.plus B)) (D₁ : Verif (Γ₂.cons A) C) (D₂ : Verif (Γ₂.cons B) C) : Verif Γ C
+  | plusE (s : Split Γ Γ₁ Γ₂) (D : Use Γ₁ (A.plus B)) (D₁ : Verif (Γ₂.cons A) C) (D₂ : Verif (Γ₂.cons B) C) : Verif Γ C
   | withI (D₁ : Verif Γ A) (D₂ : Verif Γ B) : Verif Γ (A.with B)
   | lolliI (D : Verif (Γ.cons A) B) : Verif Γ (A.lolli B)
 
@@ -271,58 +206,34 @@ inductive Use : (Γ : Ctx) → (A : Propn) → Type
   | hyp : Use (.cons .nil A) A
   | withE₁ (D : Use Γ (A.with B)) : Use Γ A
   | withE₂ (D : Use Γ (.with A B)) : Use Γ B
-  | lolliE (h : Split Γ Γ₁ Γ₂) (D : Use Γ₁ (A.lolli B)) (D₁ : Verif Γ₂ A) : Use Γ B
+  | lolliE (s : Split Γ Γ₁ Γ₂) (D : Use Γ₁ (A.lolli B)) (D₁ : Verif Γ₂ A) : Use Γ B
 
 end
 
-mutual
-
-def Verif.rename (γ : Rename Γ Γ') {A} : (D : Verif Γ A) → Verif Γ' A
-  | .uv D => .uv (D.rename γ)
-  | .oneI => let .nil := γ; .oneI
-  | .oneE h D D₁ => let ⟨_, _, γ₁, γ₂, h⟩ := γ.split h; .oneE h (D.rename γ₁) (D₁.rename γ₂)
-  | .zeroE h D => let ⟨_, _, γ₁, _, h⟩ := γ.split h; .zeroE h (D.rename γ₁)
-  | .topI => .topI
-  | .tensorI h D₁ D₂ => let ⟨_, _, γ₁, γ₂, h⟩ := γ.split h; .tensorI h (D₁.rename γ₁) (D₂.rename γ₂)
-  | .tensorE h D D₁ => let ⟨_, _, γ₁, γ₂, h⟩ := γ.split h; .tensorE h (D.rename γ₁) (D₁.rename γ₂.cons'.cons')
-  | .plusI₁ D => .plusI₁ (D.rename γ)
-  | .plusI₂ D => .plusI₂ (D.rename γ)
-  | .plusE h D D₁ D₂ => let ⟨_, _, γ₁, γ₂, h⟩ := γ.split h; .plusE h (D.rename γ₁) (D₁.rename γ₂.cons') (D₂.rename γ₂.cons')
-  | .withI D₁ D₂ => .withI (D₁.rename γ) (D₂.rename γ)
-  | .lolliI D => .lolliI (D.rename γ.cons')
-
-def Use.rename (γ : Rename Γ Γ') {A} : (D : Use Γ A) → Use Γ' A
-  | .hyp => let .cons u γ := γ; match u, γ with | .here (Γ := .nil), .nil => .hyp
-  | .withE₁ D => .withE₁ (D.rename γ)
-  | .withE₂ D => .withE₂ (D.rename γ)
-  | .lolliE h D D₁ => let ⟨_, _, γ₁, γ₂, h⟩ := γ.split h; .lolliE h (D.rename γ₁) (D₁.rename γ₂)
-
-end
-
-instance Use.instJudge : Judge Use where
-  hyp := hyp
+instance Use.judge : Judge Use where
+  transform | .mk => hyp
 
 mutual
 
-def Verif.subst (γ : Subst Use Γ Γ') {A} : (D : Verif Γ A) → Verif Γ' A
+def Verif.subst [j : Judge J] [jt : JudgeTrans J Use] {Γ Γ'} (γ : Subst J Γ Γ') {A} : (D : Verif Γ A) → Verif Γ' A
   | .uv D => .uv (D.subst γ)
   | .oneI => let .nil := γ; .oneI
-  | .oneE h D D₁ => let ⟨_, _, γ₁, γ₂, h⟩ := γ.split h; .oneE h (D.subst γ₁) (D₁.subst γ₂)
-  | .zeroE h D => let ⟨_, _, γ₁, _, h⟩ := γ.split h; .zeroE h (D.subst γ₁)
+  | .oneE s D D₁ => let ⟨_, _, s, γ₁, γ₂⟩ := γ.split s; .oneE s (D.subst γ₁) (D₁.subst γ₂)
+  | .zeroE s D => let ⟨_, _, s, γ₁, _⟩ := γ.split s; .zeroE s (D.subst γ₁)
   | .topI => .topI
-  | .tensorI h D₁ D₂ => let ⟨_, _, γ₁, γ₂, h⟩ := γ.split h; .tensorI h (D₁.subst γ₁) (D₂.subst γ₂)
-  | .tensorE h D D₁ => let ⟨_, _, γ₁, γ₂, h⟩ := γ.split h; .tensorE h (D.subst γ₁) (D₁.subst γ₂.cons'.cons')
+  | .tensorI s D₁ D₂ => let ⟨_, _, s, γ₁, γ₂⟩ := γ.split s; .tensorI s (D₁.subst γ₁) (D₂.subst γ₂)
+  | .tensorE s D D₁ => let ⟨_, _, s, γ₁, γ₂⟩ := γ.split s; .tensorE s (D.subst γ₁) (D₁.subst γ₂.lift.lift)
   | .plusI₁ D => .plusI₁ (D.subst γ)
   | .plusI₂ D => .plusI₂ (D.subst γ)
-  | .plusE h D D₁ D₂ => let ⟨_, _, γ₁, γ₂, h⟩ := γ.split h; .plusE h (D.subst γ₁) (D₁.subst γ₂.cons') (D₂.subst γ₂.cons')
+  | .plusE s D D₁ D₂ => let ⟨_, _, s, γ₁, γ₂⟩ := γ.split s; .plusE s (D.subst γ₁) (D₁.subst γ₂.lift) (D₂.subst γ₂.lift)
   | .withI D₁ D₂ => .withI (D₁.subst γ) (D₂.subst γ)
-  | .lolliI D => .lolliI (D.subst γ.cons')
+  | .lolliI D => .lolliI (D.subst γ.lift)
 
-def Use.subst (γ : Subst Use Γ Γ') {A} : (D : Use Γ A) → Use Γ' A
-  | .hyp => let .cons h D .nil := γ; match h.eq_triv₁ with | rfl => D
+def Use.subst [j : Judge J] [jt : JudgeTrans J Use] {Γ Γ'} (γ : Subst J Γ Γ') {A} : (D : Use Γ A) → Use Γ' A
+  | .hyp => let .cons s D .nil := γ; let .refl _ := s.eq_triv₁; jt.transform D
   | .withE₁ D => .withE₁ (D.subst γ)
   | .withE₂ D => .withE₂ (D.subst γ)
-  | .lolliE h D D₁ => let ⟨_, _, γ₁, γ₂, h⟩ := γ.split h; .lolliE h (D.subst γ₁) (D₁.subst γ₂)
+  | .lolliE s D D₁ => let ⟨_, _, s, γ₁, γ₂⟩ := γ.split s; .lolliE s (D.subst γ₁) (D₁.subst γ₂)
 
 end
 
@@ -337,19 +248,22 @@ def Verif.uv' (D : Use Γ A) : Verif Γ A :=
   | .with .. => withI (uv' (.withE₁ D)) (uv' (.withE₂ D))
   | .lolli .. => lolliI (uv' (.lolliE (.cons₂ .triv₁) D (uv' .hyp)))
 
+instance Verif.judge : Judge Verif where
+  transform | .mk => uv' .hyp
+
 mutual
 
 def Verif.toTrue : (D : Verif Γ A) → ND.True Γ A
   | .uv D => D.toTrue
   | .oneI => .oneI
-  | .oneE h D D₁ => .oneE h D.toTrue D₁.toTrue
-  | .zeroE h D => .zeroE h D.toTrue
+  | .oneE s D D₁ => .oneE s D.toTrue D₁.toTrue
+  | .zeroE s D => .zeroE s D.toTrue
   | .topI => .topI
-  | .tensorI h D₁ D₂ => .tensorI h D₁.toTrue D₂.toTrue
-  | .tensorE h D D₁ => .tensorE h D.toTrue D₁.toTrue
+  | .tensorI s D₁ D₂ => .tensorI s D₁.toTrue D₂.toTrue
+  | .tensorE s D D₁ => .tensorE s D.toTrue D₁.toTrue
   | .plusI₁ D => .plusI₁ D.toTrue
   | .plusI₂ D => .plusI₂ D.toTrue
-  | .plusE h D D₁ D₂ => .plusE h D.toTrue D₁.toTrue D₂.toTrue
+  | .plusE s D D₁ D₂ => .plusE s D.toTrue D₁.toTrue D₂.toTrue
   | .withI D₁ D₂ => .withI D₁.toTrue D₂.toTrue
   | .lolliI D => .lolliI D.toTrue
 
@@ -357,7 +271,7 @@ def Use.toTrue : (D : Use Γ A) → ND.True Γ A
   | .hyp => .hyp
   | .withE₁ D => .withE₁ D.toTrue
   | .withE₂ D => .withE₂ D.toTrue
-  | .lolliE h D D₁ => .lolliE h D.toTrue D₁.toTrue
+  | .lolliE s D D₁ => .lolliE s D.toTrue D₁.toTrue
 
 end
 
@@ -369,36 +283,36 @@ namespace SC
 inductive Seq : (Γ : Ctx) → (A : Propn) → Type
   | id : Seq (.cons .nil (.base P)) (.base P)
   | oneR : Seq .nil .one
-  | oneL (u : Mem .one Γ) (D : Seq (Γ.del u) C) : Seq Γ C
-  | zeroL (u : Mem .zero Γ) : Seq Γ C
+  | oneL (s : Split₁ Γ .one Γ') (D : Seq Γ' C) : Seq Γ C
+  | zeroL (s : Split₁ Γ .zero Γ') : Seq Γ C
   | topR : Seq Γ .top
-  | tensorR (h : Split Γ Γ₁ Γ₂) (D₁ : Seq Γ₁ A) (D₂ : Seq Γ₂ B) : Seq Γ (A.tensor B)
-  | tensorL (u : Mem (A.tensor B) Γ) (D : Seq (Γ.del u |>.cons A |>.cons B) C) : Seq Γ C
+  | tensorR (s : Split Γ Γ₁ Γ₂) (D₁ : Seq Γ₁ A) (D₂ : Seq Γ₂ B) : Seq Γ (A.tensor B)
+  | tensorL (s : Split₁ Γ (A.tensor B) Γ') (D : Seq (Γ'.cons A |>.cons B) C) : Seq Γ C
   | plusR₁ (D : Seq Γ A) : Seq Γ (A.plus B)
   | plusR₂ (D : Seq Γ B) : Seq Γ (.plus A B)
-  | plusL (u : Mem (A.plus B) Γ) (D₁ : Seq (Γ.del u |>.cons A) C) (D₂ : Seq (Γ.del u |>.cons B) C) : Seq Γ C
+  | plusL (s : Split₁ Γ (A.plus B) Γ') (D₁ : Seq (Γ'.cons A) C) (D₂ : Seq (Γ'.cons B) C) : Seq Γ C
   | withR (D₁ : Seq Γ A) (D₂ : Seq Γ B) : Seq Γ (A.with B)
-  | withL₁ (u : Mem (A.with B) Γ) (D : Seq (Γ.del u |>.cons A) C) : Seq Γ C
-  | withL₂ (u : Mem (.with A B) Γ) (D : Seq (Γ.del u |>.cons B) C) : Seq Γ C
+  | withL₁ (s : Split₁ Γ (A.with B) Γ') (D : Seq (Γ'.cons A) C) : Seq Γ C
+  | withL₂ (s : Split₁ Γ (.with A B) Γ') (D : Seq (Γ'.cons B) C) : Seq Γ C
   | lolliR (D : Seq (Γ.cons A) B) : Seq Γ (A.lolli B)
-  | lolliL (u : Mem (A.lolli B) Γ) (h : Split (Γ.del u) Γ₁ Γ₂) (D₁ : Seq Γ₁ A) (D₂ : Seq (Γ₂.cons B) C) : Seq Γ C
+  | lolliL (s : Split₁ Γ (A.lolli B) Γ') (s' : Split Γ' Γ₁ Γ₂) (D₁ : Seq Γ₁ A) (D₂ : Seq (Γ₂.cons B) C) : Seq Γ C
 
-def Seq.rename (γ : Rename Γ Γ') {A} : (D : Seq Γ A) → Seq Γ' A
-  | id => let .cons u γ := γ; match u, γ with | .here (Γ := .nil), .nil => id
+def Seq.rename (γ : Subst Hyp Γ Γ') {A} : (D : Seq Γ A) → Seq Γ' A
+  | id => let .cons s .mk .nil := γ; let .refl _ := s.eq_triv₁; id
   | oneR => let .nil := γ; oneR
-  | oneL u D => oneL (u.rename γ) (D.rename (γ.del u))
-  | zeroL u => zeroL (u.rename γ)
+  | oneL s D => let ⟨_, s, γ⟩ := γ.split₁ s; oneL s (D.rename γ)
+  | zeroL s => let ⟨_, s, _⟩ := γ.split₁ s; zeroL s
   | topR => topR
-  | tensorR h D₁ D₂ => let ⟨_, _, γ₁, γ₂, h⟩ := γ.split h; tensorR h (D₁.rename γ₁) (D₂.rename γ₂)
-  | tensorL u D => tensorL (u.rename γ) (D.rename (γ.del u).cons'.cons')
+  | tensorR s D₁ D₂ => let ⟨_, _, s, γ₁, γ₂⟩ := γ.split s; tensorR s (D₁.rename γ₁) (D₂.rename γ₂)
+  | tensorL s D => let ⟨_, s, γ⟩ := γ.split₁ s; tensorL s (D.rename γ.lift.lift)
   | plusR₁ D => plusR₁ (D.rename γ)
   | plusR₂ D => plusR₂ (D.rename γ)
-  | plusL u D₁ D₂ => plusL (u.rename γ) (D₁.rename (γ.del u).cons') (D₂.rename (γ.del u).cons')
+  | plusL s D₁ D₂ => let ⟨_, s, γ⟩ := γ.split₁ s; plusL s (D₁.rename γ.lift) (D₂.rename γ.lift)
   | withR D₁ D₂ => withR (D₁.rename γ) (D₂.rename γ)
-  | withL₁ u D => withL₁ (u.rename γ) (D.rename (γ.del u).cons')
-  | withL₂ u D => withL₂ (u.rename γ) (D.rename (γ.del u).cons')
-  | lolliR D => lolliR (D.rename γ.cons')
-  | lolliL u h D₁ D₂ => let ⟨_, _, γ₁, γ₂, h⟩ := (γ.del u).split h; lolliL (u.rename γ) h (D₁.rename γ₁) (D₂.rename γ₂.cons')
+  | withL₁ s D => let ⟨_, s, γ⟩ := γ.split₁ s; withL₁ s (D.rename γ.lift)
+  | withL₂ s D => let ⟨_, s, γ⟩ := γ.split₁ s; withL₂ s (D.rename γ.lift)
+  | lolliR D => lolliR (D.rename γ.lift)
+  | lolliL s s' D₁ D₂ => let ⟨_, s, γ⟩ := γ.split₁ s; let ⟨_, _, s', γ₁, γ₂⟩ := γ.split s'; lolliL s s' (D₁.rename γ₁) (D₂.rename γ₂.lift)
 
 def Seq.id' : Seq (.cons .nil A) A :=
   match A with
@@ -418,49 +332,47 @@ def Seq.sizeOf : (D : Seq Γ A) → Nat
   | tensorR _ D₁ D₂ | plusL _ D₁ D₂ | withR D₁ D₂ | lolliL _ _ D₁ D₂ => D₁.sizeOf + D₂.sizeOf + 1
 
 @[simp]
-theorem Seq.sizeOf_rename {γ : Rename Γ Γ'} (D : Seq Γ A) : (D.rename γ).sizeOf = D.sizeOf := by
+theorem Seq.sizeOf_rename (γ : Subst Hyp Γ Γ') {A} (D : Seq Γ A) : (D.rename γ).sizeOf = D.sizeOf := by
   induction D generalizing Γ' <;> simp! only [*]
-  case id => let .cons u γ := γ; match u, γ with | .here (Γ := .nil), .nil => rfl
+  case id => let .cons s .mk .nil := γ; let .refl _ := s.eq_triv₁; rfl
   case oneR => let .nil := γ; rfl
 
-def Seq.cut (h : Split Γ Γ₁ Γ₂) : (D : Seq Γ₁ A) → (E : Seq (Γ₂.cons A) C) → Seq Γ C
-  | D, id => match h.eq_triv₁ with | rfl => D
-  | oneR, oneL .here E => match h.eq_triv₂ with | rfl => E
-  | tensorR h₁ D₁ D₂, tensorL .here E => let ⟨_, h', h''⟩ := h.shift₁ h₁; cut h' D₁ (cut h''.cons₂ D₂ E)
-  | plusR₁ D, plusL .here E₁ _ => cut h D E₁
-  | plusR₂ D, plusL .here _ E₂ => cut h D E₂
-  | withR D₁ _, withL₁ .here E => cut h D₁ E
-  | withR _ D₂, withL₂ .here E => cut h D₂ E
-  | lolliR D, lolliL .here h₂ E₁ E₂ => let ⟨_, h', h''⟩ := h.shift₂ h₂; cut h' (cut h''.flip E₁ D) E₂
-  | oneL u D, E => oneL (u.ofSplit₁ h) (cut (h.del₁ u) D E)
-  | zeroL u, _ => zeroL (u.ofSplit₁ h)
-  | tensorL u D, E => tensorL (u.ofSplit₁ h) (cut (h.del₁ u).cons₁.cons₁ D E)
-  | plusL u D₁ D₂, E => plusL (u.ofSplit₁ h) (cut (h.del₁ u).cons₁ D₁ E) (cut (h.del₁ u).cons₁ D₂ E)
-  | withL₁ u D, E => withL₁ (u.ofSplit₁ h) (cut (h.del₁ u).cons₁ D E)
-  | withL₂ u D, E => withL₂ (u.ofSplit₁ h) (cut (h.del₁ u).cons₁ D E)
-  | lolliL u h₁ D₁ D₂, E => let ⟨_, h', h''⟩ := (h.del₁ u).shift₁ h₁; lolliL (u.ofSplit₁ h) h' D₁ (cut h''.cons₁ D₂ E)
-  | D, oneL (.there u) E => oneL (u.ofSplit₂ h) (cut (h.del₂ u) D E)
-  | _, zeroL (.there u) => zeroL (u.ofSplit₂ h)
+def Seq.cut (s : Split Γ Γ₁ Γ₂) : (D : Seq Γ₁ A) → (E : Seq (Γ₂.cons A) C) → Seq Γ C
+  | D, id => let .refl _ := s.eq_triv₁; D
+  | oneR, oneL .here E => let .refl _ := s.eq_triv₂; E
+  | tensorR s' D₁ D₂, tensorL .here E => let ⟨_, s, s'⟩ := s.shift₁ s'; cut s D₁ (cut s'.cons₂ D₂ E)
+  | plusR₁ D, plusL .here E₁ _ => cut s D E₁
+  | plusR₂ D, plusL .here _ E₂ => cut s D E₂
+  | withR D₁ _, withL₁ .here E => cut s D₁ E
+  | withR _ D₂, withL₂ .here E => cut s D₂ E
+  | lolliR D, lolliL .here s₂ E₁ E₂ => let ⟨_, s, s'⟩ := s.flip.shift₁ s₂.flip; cut s.flip (cut s' E₁ D) E₂
+  | oneL s' D, E => let ⟨_, s, s'⟩ := s.shift₁ s'.toSplit; oneL (.ofSplit s) (cut s' D E)
+  | zeroL s', _ => let ⟨_, s, _⟩ := s.shift₁ s'.toSplit; zeroL (.ofSplit s)
+  | tensorL s' D, E => let ⟨_, s, s'⟩ := s.shift₁ s'.toSplit; tensorL (.ofSplit s) (cut s'.cons₁.cons₁ D E)
+  | plusL s' D₁ D₂, E => let ⟨_, s, s'⟩ := s.shift₁ s'.toSplit; plusL (.ofSplit s) (cut s'.cons₁ D₁ E) (cut s'.cons₁ D₂ E)
+  | withL₁ s' D, E => let ⟨_, s, s'⟩ := s.shift₁ s'.toSplit; withL₁ (.ofSplit s) (cut s'.cons₁ D E)
+  | withL₂ s' D, E => let ⟨_, s, s'⟩ := s.shift₁ s'.toSplit; withL₂ (.ofSplit s) (cut s'.cons₁ D E)
+  | lolliL s' s'' D₁ D₂, E => let ⟨_, s, s'⟩ := s.shift₁ s'.toSplit; let ⟨_, s', s''⟩ := s'.shift₁ s''; lolliL (.ofSplit s) s' D₁ (cut s''.cons₁ D₂ E)
+  | D, oneL (.there s') E => let ⟨_, s, s'⟩ := s.flip.shift₁ s'.toSplit; oneL (.ofSplit s) (cut s'.flip D E)
+  | _, zeroL (.there s') => let ⟨_, s, _⟩ := s.flip.shift₁ s'.toSplit; zeroL (.ofSplit s)
   | _, topR => topR
-  | D, tensorR (.cons₁ h₂) E₁ E₂ => let ⟨_, h', h''⟩ := h.shift₂ h₂; tensorR h' (cut h'' D E₁) E₂
-  | D, tensorR (.cons₂ h₂) E₁ E₂ => let ⟨_, h', h''⟩ := h.flip.shift₁ h₂; tensorR h' E₁ (cut h''.flip D E₂)
-  | D, tensorL (.there u) E => tensorL (u.ofSplit₂ h) (cut (h.del₂ u).cons₂.cons₂ D (E.rename .exchange₂))
-  | D, plusR₁ E => plusR₁ (cut h D E)
-  | D, plusR₂ E => plusR₂ (cut h D E)
-  | D, plusL (.there u) E₁ E₂ => plusL (u.ofSplit₂ h) (cut (h.del₂ u).cons₂ D (E₁.rename .exchange)) (cut (h.del₂ u).cons₂ D (E₂.rename .exchange))
-  | D, withR E₁ E₂ => withR (cut h D E₁) (cut h D E₂)
-  | D, withL₁ (.there u) E => withL₁ (u.ofSplit₂ h) (cut (h.del₂ u).cons₂ D (E.rename .exchange))
-  | D, withL₂ (.there u) E => withL₂ (u.ofSplit₂ h) (cut (h.del₂ u).cons₂ D (E.rename .exchange))
-  | D, lolliR E => lolliR (cut h.cons₂ D (E.rename .exchange))
-  | D, lolliL (.there u) h₂ E₁ E₂ =>
-    match h₂ with
-    | .cons₁ h₂ => let ⟨_, h', h''⟩ := (h.del₂ u).shift₂ h₂; lolliL (u.ofSplit₂ h) h' (cut h'' D E₁) E₂
-    | .cons₂ h₂ => let ⟨_, h', h''⟩ := (h.del₂ u).flip.shift₁ h₂; lolliL (u.ofSplit₂ h) h' E₁ (cut h''.flip.cons₂ D (E₂.rename .exchange))
+  | D, tensorR (.cons₁ s') E₁ E₂ => let ⟨_, s, s'⟩ := s.flip.shift₁ s'.flip; tensorR s.flip (cut s'.flip D E₁) E₂
+  | D, tensorR (.cons₂ s') E₁ E₂ => let ⟨_, s, s'⟩ := s.flip.shift₁ s'; tensorR s E₁ (cut s'.flip D E₂)
+  | D, tensorL (.there s') E => let ⟨_, s, s'⟩ := s.flip.shift₁ s'.toSplit; tensorL (.ofSplit s) (cut s'.flip.cons₂.cons₂ D (E.rename .exchange₂))
+  | D, plusR₁ E => plusR₁ (cut s D E)
+  | D, plusR₂ E => plusR₂ (cut s D E)
+  | D, plusL (.there s') E₁ E₂ => let ⟨_, s, s'⟩ := s.flip.shift₁ s'.toSplit; plusL (.ofSplit s) (cut s'.flip.cons₂ D (E₁.rename .exchange)) (cut s'.flip.cons₂ D (E₂.rename .exchange))
+  | D, withR E₁ E₂ => withR (cut s D E₁) (cut s D E₂)
+  | D, withL₁ (.there s') E => let ⟨_, s, s'⟩ := s.flip.shift₁ s'.toSplit; withL₁ (.ofSplit s) (cut s'.flip.cons₂ D (E.rename .exchange))
+  | D, withL₂ (.there s') E => let ⟨_, s, s'⟩ := s.flip.shift₁ s'.toSplit; withL₂ (.ofSplit s) (cut s'.flip.cons₂ D (E.rename .exchange))
+  | D, lolliR E => lolliR (cut s.cons₂ D (E.rename .exchange))
+  | D, lolliL (.there s') (.cons₁ s'') E₁ E₂ => let ⟨_, s, s'⟩ := s.flip.shift₁ s'.toSplit; let ⟨_, s', s''⟩ := s'.shift₁ s''.flip; lolliL (.ofSplit s) s'.flip (cut s''.flip D E₁) E₂
+  | D, lolliL (.there s') (.cons₂ s'') E₁ E₂ => let ⟨_, s, s'⟩ := s.flip.shift₁ s'.toSplit; let ⟨_, s', s''⟩ := s'.shift₁ s''; lolliL (.ofSplit s) s' E₁ (cut s''.flip.cons₂ D (E₂.rename .exchange))
   termination_by D E => (A, D.sizeOf, E.sizeOf)
 
 def Seq.multicut : (γ : Subst Seq Γ₂ Γ₂') → ∀ {Γ₁ A}, (D : Seq (.append Γ₁ Γ₂) A) → Seq (Γ₁.append Γ₂') A
   | .nil, _, _, D => D
-  | .cons h D' γ, _, _, D => (multicut γ (Ctx.append_append ▸ cut .append D' D)).rename (h.rename.append.comp .appendSwap)
+  | .cons s D' γ, _, _, D => (Ctx.append_append ▸ multicut γ (cut (.append₂ (.flip .mkAppend)) D' D)).rename (.append .id s.toSubst)
 
 def Seq.subst (γ : Subst Seq Γ Γ') {A} (D : Seq Γ A) : Seq Γ' A :=
   (Ctx.nil_append ▸ multicut γ (Γ₁ := .nil) (A := A) (Ctx.nil_append ▸ D) :)
@@ -468,38 +380,38 @@ def Seq.subst (γ : Subst Seq Γ Γ') {A} (D : Seq Γ A) : Seq Γ' A :=
 def Seq.toVerif : (D : Seq Γ A) → VU.Verif Γ A
   | id => .uv .hyp
   | oneR => .oneI
-  | oneL u D => .oneE (.ofMem u) .hyp D.toVerif
-  | zeroL u => .zeroE (.ofMem u) .hyp
+  | oneL s D => .oneE s.toSplit .hyp D.toVerif
+  | zeroL s => .zeroE s.toSplit .hyp
   | topR => .topI
-  | tensorR h D₁ D₂ => .tensorI h D₁.toVerif D₂.toVerif
-  | tensorL u D => .tensorE (.ofMem u) .hyp D.toVerif
+  | tensorR s D₁ D₂ => .tensorI s D₁.toVerif D₂.toVerif
+  | tensorL s D => .tensorE s.toSplit .hyp D.toVerif
   | plusR₁ D => .plusI₁ D.toVerif
   | plusR₂ D => .plusI₂ D.toVerif
-  | plusL u D₁ D₂ => .plusE (.ofMem u) .hyp D₁.toVerif D₂.toVerif
+  | plusL s D₁ D₂ => .plusE s.toSplit .hyp D₁.toVerif D₂.toVerif
   | withR D₁ D₂ => .withI D₁.toVerif D₂.toVerif
-  | withL₁ u D => D.toVerif.subst (.cons (.ofMem u) (.withE₁ .hyp) .id)
-  | withL₂ u D => D.toVerif.subst (.cons (.ofMem u) (.withE₂ .hyp) .id)
+  | withL₁ s D => D.toVerif.subst (.cons s.toSplit (VU.Use.withE₁ .hyp) .id)
+  | withL₂ s D => D.toVerif.subst (.cons s.toSplit (VU.Use.withE₂ .hyp) .id)
   | lolliR D => .lolliI D.toVerif
-  | lolliL u h D₁ D₂ => let ⟨_, h, h'⟩ := (Split.ofMem u).shift₂ h; D₂.toVerif.subst (.cons h (.lolliE h' .hyp D₁.toVerif) .id)
+  | lolliL s s' D₁ D₂ => let ⟨_, s, s'⟩ := s.toSplit.flip.shift₁ s'.flip; D₂.toVerif.subst (.cons s.flip (VU.Use.lolliE s'.flip .hyp D₁.toVerif) .id)
 
 end SC
 
 def ND.True.toSeq : (D : True Γ A) → SC.Seq Γ A
   | hyp => .id'
   | oneI => .oneR
-  | oneE h D D₁ => .cut h D.toSeq (.oneL .here D₁.toSeq)
-  | zeroE h D => .cut h D.toSeq (.zeroL .here)
+  | oneE s D D₁ => .cut s D.toSeq (.oneL .here D₁.toSeq)
+  | zeroE s D => .cut s D.toSeq (.zeroL .here)
   | topI => .topR
-  | tensorI h D₁ D₂ => .tensorR h D₁.toSeq D₂.toSeq
-  | tensorE h D D₁ => .cut h D.toSeq (.tensorL .here D₁.toSeq)
+  | tensorI s D₁ D₂ => .tensorR s D₁.toSeq D₂.toSeq
+  | tensorE s D D₁ => .cut s D.toSeq (.tensorL .here D₁.toSeq)
   | plusI₁ D => .plusR₁ D.toSeq
   | plusI₂ D => .plusR₂ D.toSeq
-  | plusE h D D₁ D₂ => .cut h D.toSeq (.plusL .here D₁.toSeq D₂.toSeq)
+  | plusE s D D₁ D₂ => .cut s D.toSeq (.plusL .here D₁.toSeq D₂.toSeq)
   | withI D₁ D₂ => .withR D₁.toSeq D₂.toSeq
   | withE₁ D => .cut .triv₁ D.toSeq (.withL₁ .here .id')
   | withE₂ D => .cut .triv₁ D.toSeq (.withL₂ .here .id')
   | lolliI D => .lolliR D.toSeq
-  | lolliE h D D₁ => .cut h D.toSeq (.lolliL .here .triv₁ D₁.toSeq .id')
+  | lolliE s D D₁ => .cut s D.toSeq (.lolliL .here .triv₁ D₁.toSeq .id')
 
 def VU.Verif.subst' (γ : Subst Verif Γ Γ') {A} (D : Verif Γ A) : Verif Γ' A :=
-  (D.toTrue.toSeq.subst (γ.map fun D => D.toTrue.toSeq)).toVerif
+  (D.toTrue.toSeq.subst (γ.map ⟨fun D => D.toTrue.toSeq⟩)).toVerif
